src/tls/AEAD_GCM.fst
@@ -279,7 +279,7 @@ val decrypt: #i:id -> d:reader i -> ad:adata i -> c:cipher i
     /\ (match res with
        | None -> modifies Set.empty h0 h1
        | _    -> modifies_one d.region h0 h1
-                /\ modifies_ref d.region (Set.singleton (Heap.addr_of (as_ref ctr_counter_as_hsref))) h0.h h1.h
+                /\ modifies_ref d.region (Set.singleton (Heap.addr_of (as_ref ctr_counter_as_hsref))) h0 h1
 	        /\ m_sel h1 (ctr d.counter) === j + 1)))
 
 #set-options "--z3rlimit 100 --max_fuel 0 --initial_fuel 1 --initial_ifuel 0 --max_ifuel 1"
