src/tls/StAE.fst
@@ -198,7 +198,7 @@ let incrementable (#i:id) (#rw:rw) (s:state i rw) (h:mem) =
 val frame_fragments : #i:id -> #rw:rw -> st:state i rw -> h0:mem -> h1:mem -> s:Set.set rid
   -> Lemma
     (requires modifies s h0 h1
-	      /\ Map.contains h0.h (log_region st)
+	      /\ Map.contains h0 (log_region st)
 	      /\ not (Set.mem (log_region st) s))
     (ensures authId i ==> fragments st h0 == fragments st h1)
 let frame_fragments #i #rw st h0 h1 s = ()
@@ -207,7 +207,7 @@ let frame_fragments #i #rw st h0 h1 s = ()
 val frame_seqnT : #i:id -> #rw:rw -> st:state i rw -> h0:mem -> h1:mem -> s:Set.set rid
 	       -> Lemma
     (requires modifies s h0 h1
-    	  /\ Map.contains h0.h (region st)
+    	  /\ Map.contains h0 (region st)
 	      /\ not (Set.mem (region st) s))
     (ensures seqnT st h0 = seqnT st h1)
 let frame_seqnT #i #rw st h0 h1 s = ()
@@ -217,11 +217,11 @@ let trigger_frame (h:mem) = True
 let frame_f (#a:Type) (f:mem -> GTot a) (h0:mem) (s:Set.set rid) =
   forall h1.{:pattern trigger_frame h1}
         trigger_frame h1
-        /\ (HS.equal_on s h0.h h1.h ==> f h0 == f h1)
+        /\ (HS.equal_on s h0 h1 ==> f h0 == f h1)
 
 val frame_seqT_auto: i:id -> rw:rw -> s:state i rw -> h0:mem -> h1:mem ->
-  Lemma (requires   HS.equal_on (Set.singleton (region s)) h0.h h1.h
-		  /\ Map.contains h0.h (region s))
+  Lemma (requires   HS.equal_on (Set.singleton (region s)) h0 h1
+		  /\ Map.contains h0 (region s))
         (ensures seqnT s h0 = seqnT s h1)
 	[SMTPat (seqnT s h0);
 	 SMTPat (seqnT s h1)]
@@ -229,8 +229,8 @@ val frame_seqT_auto: i:id -> rw:rw -> s:state i rw -> h0:mem -> h1:mem ->
 let frame_seqT_auto i rw s h0 h1 = ()
 
 val frame_fragments_auto: i:id{authId i} -> rw:rw -> s:state i rw -> h0:mem -> h1:mem ->
-  Lemma (requires    HS.equal_on (Set.singleton (log_region s)) h0.h h1.h
-		  /\ Map.contains h0.h (log_region s))
+  Lemma (requires    HS.equal_on (Set.singleton (log_region s)) h0 h1
+		  /\ Map.contains h0 (log_region s))
         (ensures fragments s h0 == fragments s h1)
 	[SMTPat (fragments s h0);
 	 SMTPat (fragments s h1)]
@@ -242,7 +242,7 @@ let frame_fragments_auto i rw s h0 h1 = ()
 //Experimenting with reads clauses: probably unnecessary
 ////////////////////////////////////////////////////////////////////////////////
 let reads (s:Set.set rid) (a:Type) =
-    f: (h:mem -> GTot a){forall h1 h2. (HS.equal_on s h1.h h2.h /\ Set.subset s (Map.domain h1.h))
+    f: (h:mem -> GTot a){forall h1 h2. (HS.equal_on s h1 h2 /\ Set.subset s (Map.domain h1))
 				  ==> f h1 == f h2}
 
 (*
@@ -253,9 +253,9 @@ let fragments' #i #rw s = fun h -> fragments #i #rw s h
 (*------------------------------------------------------------------*)
 let genPost (#i:id) parent h0 (w:writer i) h1 =
   let r = region #i #Writer w in
-  HS.modifies Set.empty h0.h h1.h /\
+  HS.modifies Set.empty h0 h1 /\
   HS.extends r parent /\
-  stronger_fresh_region r h0 h1 /\
+  fresh_region r h0 h1 /\
   color r = color parent /\
   seqnT #i #Writer w h1 = 0 /\
   (authId i ==> fragments #i #Writer w h1 == Seq.createEmpty) // we need to re-apply #i knowning authId
@@ -275,13 +275,13 @@ let gen parent i =
 val genReader: parent:rgn -> #i:id -> w:writer i -> ST (reader i)
   (requires (fun h0 -> 
     witnessed (region_contains_pred parent) /\
-    HyperHeap.disjoint parent (region #i #Writer w))) //16-04-25  we may need w.region's parent instead
+    disjoint parent (region #i #Writer w))) //16-04-25  we may need w.region's parent instead
   (ensures  (fun h0 (r:reader i) h1 ->
                modifies Set.empty h0 h1 /\
                log_region r = region #i #Writer w /\
                extends (region r) parent /\
 	       color (region r) = color parent /\
-               stronger_fresh_region (region r) h0 h1 /\
+               fresh_region (region r) h0 h1 /\
                //op_Equality #(log_ref w.region i) w.log r.log /\
                seqnT r h1 = 0))
 // encryption, recorded in the log; safe instances are idealized
@@ -289,11 +289,11 @@ let genReader parent #i w =
   match w with
   | Stream _ w ->
     lemma_ID13 i;
-    assume(StreamAE.(HyperHeap.disjoint parent (AEADProvider.region #i w.aead)));
+    assume(StreamAE.(disjoint parent (AEADProvider.region #i w.aead)));
     Stream () (StreamAE.genReader parent #i w)
   | StLHAE _ w ->
     lemma_ID12 i;
-    assume(AEAD_GCM.(HyperHeap.disjoint parent (AEADProvider.region #i w.aead)));
+    assume(AEAD_GCM.(disjoint parent (AEADProvider.region #i w.aead)));
     StLHAE () (StLHAE.genReader parent #i w)
 
 
